implement typed assign-once prophecy variables

src/goose_lang/lib/proph/proph.v
@@ -1,5 +1,5 @@
 From Perennial.goose_lang Require Import notation typing.
-From Perennial.goose_lang Require Import proofmode lifting.
+From Perennial.goose_lang Require Import proofmode lifting lib.into_val.
 From Perennial.goose_lang.lib Require Export proph.impl.
 
 Set Default Proof Using "Type".
@@ -8,10 +8,12 @@ Section goose_lang.
 Context `{ffi_sem: ffi_semantics} `{!ffi_interp ffi} `{!heapGS Σ}.
 Context {ext_ty: ext_types ext}.
 
+(** list-based prophecy variables (the most general underlying primitive) *)
+
 Theorem wp_NewProph_list :
   {{{ True }}}
     NewProph #()
-  {{{ pvs (p : proph_id), RET #p; proph p pvs }}}.
+  {{{ (p : proph_id) pvs, RET #p; proph p pvs }}}.
 Proof.
   iIntros (Φ) "_ HΦ". wp_lam.
   wp_apply wp_new_proph. auto.
@@ -25,5 +27,44 @@ Proof.
   iIntros (Φ) "Hp HΦ". wp_lam.
   wp_apply (wp_resolve_proph with "Hp"). auto.
 Qed.
+
+(** typed assign-once prophecy variables *)
+Section once.
+  Context `{!IntoVal T}.
+
+  Definition proph_once (p : proph_id) (x : T) : iProp Σ :=
+    ∃ pvs : list val, proph p pvs ∗
+               ⌜match v ← head pvs; from_val v with
+                | Some x' => x=x'
+                | None => True
+                end⌝.
+
+  Theorem wp_NewProph_once :
+    {{{ True }}}
+      NewProph #()
+    {{{ (p : proph_id) (x : T), RET #p; proph_once p x }}}.
+  Proof.
+    iIntros (Φ) "_ HΦ". iApply wp_NewProph_list; first done.
+    iIntros "!> %p %pvs Hp".
+    iApply ("HΦ" $! p (default (IntoVal_def T) (v ← head pvs; from_val v))).
+    iExists pvs. iFrame. iPureIntro.
+    destruct (head pvs); simpl; last done.
+    destruct (from_val v); done.
+  Qed.
+
+  Theorem wp_ResolveProph_once (p : proph_id) (x y : T) v :
+    from_val v = Some y →
+    {{{ proph_once p x }}}
+      ResolveProph (#p) (Val v)
+    {{{ RET (LitV LitUnit); ⌜x = y⌝ }}}.
+  Proof.
+    iIntros (Hv Φ) "(%pvs & Hp & %Hpvs) HΦ".
+    iApply (wp_ResolveProph_list with "Hp").
+    iIntros "!> %pvs' [%Hpvs' _]". iApply "HΦ". iPureIntro.
+    subst pvs. simpl in Hpvs.
+    rewrite Hv in Hpvs. done.
+  Qed.
+
+End once.
 
 End goose_lang.
